

2.5 The Chain Rule

Let $f(x)$ and $g(x)$ be differentiable functions.

$$\text{If } P(x) = f(x) \cdot g(x)$$

and

$$Q(x) = \frac{f(x)}{g(x)}$$

then

$$P'(x) = g(x)f'(x) + f(x)g'(x)$$

and

$$Q'(x) = \frac{g(x)f'(x) - f(x)g'(x)}{[g(x)]^2}$$

EX: Which of the following functions do we know how to differentiate?

(a) $\sin(x) \cdot e^x$ ✓

(b) $\frac{\sin(x)}{e^x}$ ✓

(c) $e^{\sin(x)}$ ← how do we do this? The chain rule

1
Notice this is a composition of two functions.

Def: Let $f(x)$ and $g(x)$ be functions.
The composite function $(f \circ g)(x)$ is given by

$$(f \circ g)(x) = f(g(x))$$

EX: For the following composite functions identify the inner function + outer function.

$g(x)$ $f(x)$

① $\sqrt{x^2 + 1}$ $g(x) = x^2 + 1$ $f(x) = \sqrt{x}$

$$f(g(x)) = \sqrt{x^2 + 1}$$

② $(x^3 - 1)^{100}$ $g(x) = x^3 - 1$ $f(x) = x^{100}$

$$f(g(x)) = (x^3 - 1)^{100}$$

③ $\cos(x^2)$ $g(x) = x^2$ $f(x) = \cos x$

$$f(g(x)) = \cos(x^2)$$

④ $e^{\sin x}$ $g(x) = \sin x$ $f(x) = e^x$

$$f(g(x)) = e^{\sin x}$$

⑤ $\cos^2 x$ $g(x) = \cos x$ $f(x) = x^2$
 \parallel
 $(\cos(x))^2$

$$f(g(x)) = (\cos(x))^2$$

The Chain Rule

Let $f(x)$ and $g(x)$ be functions and let $F(x) = f(g(x))$. Suppose g is differentiable at x and f is diff. at $g(x)$. Then

$$F'(x) = f'(g(x)) g'(x).$$

"Proof": \rightarrow single pt
 Full pf in book

Consider the limit definition of the derivative of $f(x)$ at $x=a$

$$f'(a) = \lim_{x \rightarrow a} \frac{f(x) - f(a)}{x - a}$$

by substitution

$$f'(g(a)) = \lim_{g(x) \rightarrow g(a)} \frac{f(g(x)) - f(g(a))}{g(x) - g(a)}$$

Also

$$g'(a) = \lim_{x \rightarrow a} \frac{g(x) - g(a)}{x - a}$$

multiplying these together gives

$$f'(g(a)) g'(a)$$

$$= \lim_{g(x) \rightarrow g(a)} \frac{f(g(x)) - f(g(a))}{g(x) - g(a)} \lim_{x \rightarrow a} \frac{g(x) - g(a)}{x - a}$$

Since $g(x)$ is continuous

$$g(x) \rightarrow g(a) \text{ as } x \rightarrow a$$

So

$$= \lim_{x \rightarrow a} \frac{f(g(x)) - f(g(a))}{\cancel{g(x) - g(a)}} \cdot \frac{\cancel{g(x) - g(a)}}{(x - a)}$$

$$= \lim_{x \rightarrow a} \frac{f(g(x)) - f(g(a))}{x - a}$$

$$= (f \circ g)'(a). \checkmark$$

Let's check what we know!

EX1: use power rule + chain rule to compute derivative of $(x^2)^2$

power rule:

$$\frac{d}{dx}(x^4) = 4x^3$$

Chain rule:

$$f(g(x)) = (x^2)^2$$

$$g(x) = x^2 \quad f(x) = x^2$$

$$g'(x) = 2x \quad f'(x) = 2x$$

$$f'(g(x))g'(x) = 2(x^2)2x = 4x^3$$

Ex 2: use the product rule + chain rule to compute the derivative of $\cos^2 x$

product of $\cos x \cdot \cos x$

$$\cos x (-\sin x) + \cos x (-\sin x)$$

$$= -2 \cos x \sin x$$

chain

$$g(x) = \cos x$$

$$g'(x) = -\sin x$$

$$f(x) = x^2$$

$$f'(x) = 2x$$

$$f'(g(x))g'(x)$$

$$= f'(\cos x) \cdot (-\sin x)$$

$$= -2 \cos x \sin x$$

Ex 3: Find derivative of $\sqrt{x^2+1}$

$$g(x) = x^2+1$$

$$g'(x) = 2x$$

$$f(x) = \sqrt{x}$$

$$f'(x) = \frac{1}{2} x^{-1/2} = \frac{1}{2\sqrt{x}}$$

$$\begin{aligned}
 & f'(g(x))g'(x) \\
 &= f'(x^2+1) \cdot 2x \\
 &= \frac{1}{2\sqrt{x^2+1}} \cdot 2x = \frac{x}{\sqrt{x^2+1}}
 \end{aligned}$$

Ex 4: Let $h(x) = \sec(x^2 e^x)$

compute $h'(x)$.

$$g(x) = x^2 e^x \xrightarrow{\text{prod. rule}} g'(x) = 2xe^x + e^x x^2$$

$$f(x) = \sec(x) \quad f'(x) = \sec x \tan x$$

$$\begin{aligned}
 h'(x) &= f'(g(x))g'(x) \\
 &= f'(x^2 e^x) \cdot (2xe^x + e^x x^2) \\
 &= \sec(x^2 e^x) \tan(x^2 e^x) (2xe^x + e^x x^2)
 \end{aligned}$$

Useful special case:

$$\frac{d}{dx} [g(x)]^n = n[g(x)]^{n-1} g'(x)$$

EX:

$$\frac{d}{dx} (3(x^2+4)^{100}) = 3 \cdot 100(x^2+4)^{99} (2x)$$

or

$$\frac{d}{d\theta} (\cos(\theta))^4 = 4(\cos \theta)^3 (-\sin \theta)$$